For the 4-vectors 
\[
w = 
\begin{bmatrix}
-2 \\
2 \\
1 \\
1
\end{bmatrix}
\quad \text{and} \quad
w' = 
\begin{bmatrix}
3 \\
4 \\
0 \\
1
\end{bmatrix},
\]
show that the collection of vectors
\[
V = \left\{ 
x = 
\begin{bmatrix}
x_1 \\
x_2 \\
x_3 \\
x_4
\end{bmatrix} 
\in \mathbb{R}^4 : x \cdot w = 0, \, x \cdot w' = 0
\right\}
\]
is a linear subspace of $\mathbb{R}^4$ in each of the following ways:

\begin{enumerate}
    \item[(a)] For $x \in V$, solve for each of $x_3$ and $x_4$ in terms of $x_1$ and $x_2$ to write $V$ as a span of two vectors;
    \item[(b)] For $x \in V$, solve for each of $x_1$ and $x_4$ in terms of $x_2$ and $x_3$ to write $V$ as a span of two vectors.
\end{enumerate}

Solution:
\begin{enumerate}


\item[(a)] For \(w\),
\[
w \cdot x = -2x_1 + 2x_2 + x_3 + x_4 = 0 \quad \Rightarrow \quad x_3 + x_4 = 2x_1 - 2x_2 \tag{1}
\]
For \(w'\),
\[
w' \cdot x = 3x_1 + 4x_2 + x_4 = 0 \quad \Rightarrow \quad x_4 = -3x_1 - 4x_2 \tag{2}
\]
Substitute \(x_4\) from (2) into (1):
\[
x_3 + (-3x_1 - 4x_2) = 2x_1 - 2x_2
\]
\[
x_3 = 5x_1 + 2x_2 \tag{3}
\]
Thus, the components of \(x\) are:
\[
x_3 = 5x_1 + 2x_2, \quad x_4 = -3x_1 - 4x_2
\]
Substitute these into \(x\):
\[
x =
\begin{bmatrix}
x_1 \\
x_2 \\
5x_1 + 2x_2 \\
-3x_1 - 4x_2
\end{bmatrix}
= x_1
\begin{bmatrix}
1 \\
0 \\
5 \\
-3
\end{bmatrix}
+ x_2
\begin{bmatrix}
0 \\
1 \\
2 \\
-4
\end{bmatrix}
\]
The basis vectors are:
\[
\begin{bmatrix}
1 \\
0 \\
5 \\
-3
\end{bmatrix}, \quad
\begin{bmatrix}
0 \\
1 \\
2 \\
-4
\end{bmatrix}.
\]

\item[(b)] For \(w\),
\[
w \cdot x = -2x_1 + 2x_2 + x_3 + x_4 = 0 \quad \Rightarrow \quad x_4 = -2x_1 + 2x_2 - x_3 \tag{4}
\]
For \(w'\),
\[
w' \cdot x = 3x_1 + 4x_2 + x_4 = 0 \quad \Rightarrow \quad x_4 = -3x_1 - 4x_2 \tag{5}
\]
Equating \(x_4\) from (4) and (5):
\[
-2x_1 + 2x_2 - x_3 = -3x_1 - 4x_2
\]
Simplify:
\[
x_1 + 6x_2 - x_3 = 0 \quad \Rightarrow \quad x_1 = -6x_2 + x_3 \tag{6}
\]
Substitute \(x_1\) from (6) into (4):
\[
x_4 = -2(-6x_2 + x_3) + 2x_2 - x_3
\]
\[
x_4 = 12x_2 - 2x_3 + 2x_2 - x_3
\]
\[
x_4 = 14x_2 - 3x_3 \tag{7}
\]
Thus, the components of \(x\) are:
\[
x_1 = -6x_2 + x_3, \quad x_4 = 14x_2 - 3x_3
\]
Substitute these into \(x\):
\[
x =
\begin{bmatrix}
-6x_2 + x_3 \\
x_2 \\
x_3 \\
14x_2 - 3x_3
\end{bmatrix}
= x_2
\begin{bmatrix}
-6 \\
1 \\
0 \\
14
\end{bmatrix}
+ x_3
\begin{bmatrix}
1 \\
0 \\
1 \\
-3
\end{bmatrix}
\]
The basis vectors are:
\[
\begin{bmatrix}
-6 \\
1 \\
0 \\
14
\end{bmatrix}, \quad
\begin{bmatrix}
1 \\
0 \\
1 \\
-3
\end{bmatrix}.
\]

\end{enumerate}