

For 
\[
v = 
\begin{bmatrix}
1 \\
1 \\
1
\end{bmatrix}
\quad \text{and} \quad
w = 
\begin{bmatrix}
4 \\
2 \\
1
\end{bmatrix},
\]
find scalars $a$, $b$, $c$ so that
\[
\text{span}(v, w) = \left\{
\begin{bmatrix}
x \\
y \\
z
\end{bmatrix} \in \mathbb{R}^3 : ax + by + cz = 0
\right\}.
\]

For 
\[
v = 
\begin{bmatrix}
1 \\
1 \\
1
\end{bmatrix}
\quad \text{and} \quad
w = 
\begin{bmatrix}
4 \\
2 \\
1
\end{bmatrix},
\]
find scalars $a$, $b$, $c$ so that
\[
\text{span}(v, w) = \left\{
\begin{bmatrix}
x \\
y \\
z
\end{bmatrix} \in \mathbb{R}^3 : ax + by + cz = 0
\right\}.
\]

Here 
ax + by + cz = 0

From \[
v = 
\begin{bmatrix}
1 \\
1 \\
1
\end{bmatrix}
\]
we have 
\[
a(1) + 1(b) + 1(c) = 0
\]
\[
b = -(a+c)
\]

From \[
w = 
\begin{bmatrix}
4 \\
2 \\
1
\end{bmatrix}
\]
we have 
\[
a(4) + 2(b) + 1(c) = 0
\]
\[
c = -(4a+2b)
\]
Therefore we have scalars a,b,c such that 
\[
 b= -(a+c)
 \]
\[ c = -(4a+2b)
\]
Substituting a =1 and solving for b and c we get
\[
c=2
\]
\[
b =-3
\]
Substituting we have 
\[
1(x) -3(y) + 2(z) = 0
\]

From \[
v = 
\begin{bmatrix}
1 \\
1 \\
1
\end{bmatrix}
\]
\[
1(x)-3(y) + 2(z) = 0
\]
we have 
\[
1(1) -3(1) + 2(1) = 3 - 3 =0
\]


From \[
w = 
\begin{bmatrix}
4 \\
2 \\
1
\end{bmatrix}
\]

we have
\[
1(x) -3(y) + 2(z) = 0
\]
\[
1(4) + -3(2) + 2(1)
\]
\[
= 6 - 6 = 0
\]
The resulting triplets work.