For 
\[
v = 
\begin{bmatrix}
2 \\
0 \\
1
\end{bmatrix}
\quad \text{and} \quad
w = 
\begin{bmatrix}
-1 \\
1 \\
3
\end{bmatrix},
\]
find scalars $a$, $b$, $c$ so that
\[
\text{span}(v, w) = \left\{
\begin{bmatrix}
x \\
y \\
z
\end{bmatrix} \in \mathbb{R}^3 : ax + by + cz = 0
\right\}.
\]

Here 
ax + by + cz = 0

From \[
v = 
\begin{bmatrix}
2 \\
0 \\
1
\end{bmatrix}
\]
we have 
\[
a(2) + 0(b) + 1(c) = 0
\]
\[
c = -2(a)
\]

From \[
w = 
\begin{bmatrix}
-1 \\
1 \\
3
\end{bmatrix}
\]
we have 
\[
a(-1) + 1(b) + 3(c) = 0
\]
\[
b = a-3c
\]
Therefore we have scalars a,b,c such that 
\[
 b= a-3c
 \]
\[ c = -2a
\]
Substituting a =1
\[
c=-2
\]
\[
b = 1-3(-2.1) = 7
\]
Substituting we have 
\[
1(x) + 7(y) + -2(z) = 0
\]

From \[
v = 
\begin{bmatrix}
2 \\
0 \\
1
\end{bmatrix}
\]
\[
1(x) + 7(y) + -2(z) = 0
\]
we have 
\[
1(2) + 7(0) + -2(1) = 2 - 2 =0
\]


From \[
w = 
\begin{bmatrix}
-1 \\
1 \\
3
\end{bmatrix}
\]

we have
\[
1(x) + 7(y) + -2(z) = 0
\]
\[
1(-1) + 7(1) + -2(3) 
\]
\[
= -1 + 7 + -6 = -7 + 7 = 0
\]
The resulting triplets work.