Use Theorem 4.2.5 to determine the dimension (1, 2, or 3) of each of the following linear subspaces in $\mathbb{R}^3$. Show the work to justify your answer.

\begin{enumerate}
    \item[(a)] $\text{span}(\mathbf{v}, \mathbf{w})$ for 
    \[
    \mathbf{v} =
    \begin{bmatrix}
    -2 \\ 1 \\ 1
    \end{bmatrix},
    \quad
    \mathbf{w} =
    \begin{bmatrix}
    1 \\ 1 \\ 1
    \end{bmatrix}.
    \]
    \item[(b)] $\text{span}(\mathbf{v'}, \mathbf{w'})$ for 
    \[
    \mathbf{v'} =
    \begin{bmatrix}
    3 \\ 6 \\ -2
    \end{bmatrix},
    \quad
    \mathbf{w'} =
    \begin{bmatrix}
    -2 \\ -4 \\ 2
    \end{bmatrix}.
    \]
    \item[(c)] $\text{span}(\mathbf{v''}, \mathbf{w''},\mathbf{u''})$ for 
    \[
    \mathbf{v''} =
    \begin{bmatrix}
    1 \\ -2 \\ 3
    \end{bmatrix},
    \quad
    \mathbf{w''} =
    \begin{bmatrix}
    4 \\ 0 \\ 2
    \end{bmatrix},
    \quad
    \mathbf{u''} =
    \begin{bmatrix}
    3 \\ -2 \\ 4
    \end{bmatrix}.
    \]
\end{enumerate}

Solution:

\begin{enumerate}
    \item[(a)] $\text{span}(\mathbf{v}, \mathbf{w})$ for 
    \[
    \mathbf{v} =
    \begin{bmatrix}
    -2 \\ 1 \\ 1
    \end{bmatrix},
    \quad
    \mathbf{w} =
    \begin{bmatrix}
    1 \\ 1 \\ 1
    \end{bmatrix}.
    \]

    Here check if we can combine u and v such that they cancel out each other.
    This can be checked by finding out a , b such that 
    \[
    a.v + b.w = 0
    \]
    a.v  means we are stretching (or shrinking) v by a. 
    similar for b.w
    by combining a.v+b.w, we get a new vector if this new vector is 0 then they cancel each other.
    If we find non-zero values of a and b such a.v+b.w  is 0 then it means v, w are linearly dependent.  If the only solution is a=0 and b=0 then then v, w are linearly independent and v and we point to different directions.

    \[
     a.v + b.w = 0
    \]
    \[
     a.\begin{bmatrix}
    -2 \\ 1 \\ 1
    \end{bmatrix} + b.\begin{bmatrix}
    1 \\ 1 \\ 1
    \end{bmatrix}
     = 0
    \]
    This gives
    \[
    -2a +b =0
    \]
    \[
    a +b =0
    \]
    \[
    a +b =0
    \]
    Substituting 
    \[
    a=-b
    \]
    \[
    -2(-b)+b=0
    \]
    Therefore
    \[
    b=0
    \]
    \[
    a=0
    \]
    This means v and w are independent.  Together v and w span a plane which has dimension 2.

    
    
    \item[(b)] $\text{span}(\mathbf{v'}, \mathbf{w'})$ for 
    \[
    \mathbf{v'} =
    \begin{bmatrix}
    3 \\ 6 \\ -2
    \end{bmatrix},
    \quad
    \mathbf{w'} =
    \begin{bmatrix}
    -2 \\ -4 \\ 2
    \end{bmatrix}.
    \]

    Similar to (a) we have 
    a.v + b.w = 0
    \[
    a.\begin{bmatrix}
    3 \\ 6 \\ -2
    \end{bmatrix} + b.\begin{bmatrix}
    -2 \\ -4 \\ 2
    \end{bmatrix} = 0
    \]

   Now we have
    \[
      3a - 2b =0 
    \]
    \[
      6a - 4b =0 
    \]
    \[
      -2a + 2b =0 
    \]
    Substituting
    \[
    a = b
    \]
    we have 
    \[
    6(b)-4b=0
    \]
    From this we have
     \[
    b=0
    \]
     \[
    a=0
    \]

   This means v' and w' are independent.  Together v' and w' span a plane which has dimension 2.
    
    \item[(c)] $\text{span}(\mathbf{v''}, \mathbf{w''},\mathbf{u''})$ for 
    \[
    \mathbf{v''} =
    \begin{bmatrix}
    1 \\ -2 \\ 3
    \end{bmatrix},
    \quad
    \mathbf{w''} =
    \begin{bmatrix}
    4 \\ 0 \\ 2
    \end{bmatrix},
    \quad
    \mathbf{u''} =
    \begin{bmatrix}
    3 \\ -2 \\ 4
    \end{bmatrix}.
    \]
    Similar to (b) we have

    a.v'' + b.w'' + c.u'' = 0
    \[
    a.\begin{bmatrix}
    1 \\ -2 \\ 3
    \end{bmatrix} 
    + b .\begin{bmatrix}
    4 \\ 0 \\ 2
    \end{bmatrix}
    + c . \begin{bmatrix}
    3 \\ -2 \\ 4
    \end{bmatrix} = 0
    \]
    \[
    a+3b+3c = 0
    \]
    \[
    -2a-2c = 0
    \]
     \[
    3a+2b+4c = 0
    \]
    Substituting 
    \[
    a = c 
    \]
    \[
    c+3b+3c = 0
    \]
    \[
    b=\frac{-4}{3}c
    \]
    \[
    3c+2.\frac{-4}{3}c+4c=0
    \]
    \[
    a=0
    \]
    \[
    b=0
    \]
    \[
    c=0
    \]
    This means v'', w'' and u'' are independent and dimension is 3
\end{enumerate}

